Tests.lean
@@ -2,11 +2,13 @@ import SubVerso.Highlighting
 import SubVerso.Examples
 import SubVerso.Examples.Env
 import SubVerso.Examples.Slice
+import SubVerso.Module
 import SubVerso.Helper.Netstring
 import Lean.Data.Json
 import Lean.Data.NameMap
 
 open SubVerso.Examples (loadExamples Example)
+open SubVerso.Module (ModuleItem)
 open Lean.FromJson (fromJson?)
 
 open SubVerso
@@ -163,6 +165,84 @@ def testNetstrings := do
     longStr := s!"{i}({longStr}{longStr})"
   testNetstring longStr
 
+-- Loads a module. To work well, it really should lock the toolchain file, but that's not available
+-- in all targeted versions, so it's just part of these tests. See Verso for a version to use in
+-- documents.
+open System in
+def loadModuleContent (projectDir : String) (mod : String) : IO (Array ModuleItem) := do
+
+  let projectDir : FilePath := projectDir
+
+  -- Validate that the path is really a Lean project
+  let lakefile := projectDir / "lakefile.lean"
+  let lakefile' := projectDir / "lakefile.toml"
+  if !(← lakefile.pathExists) && !(← lakefile'.pathExists) then
+    throw <| .userError s!"Neither {lakefile} nor {lakefile'} exist, couldn't load project"
+  let toolchainfile := projectDir / "lean-toolchain"
+  let toolchain ← do
+      if !(← toolchainfile.pathExists) then
+        throw <| .userError s!"File {toolchainfile} doesn't exist, couldn't load project"
+      pure (← IO.FS.readFile toolchainfile).trim
+
+  -- Kludge: remove variables introduced by Lake. Clearing out DYLD_LIBRARY_PATH and
+  -- LD_LIBRARY_PATH is useful so the version selected by Elan doesn't get the wrong shared
+  -- libraries.
+  let lakeVars :=
+    #["LAKE", "LAKE_HOME", "LAKE_PKG_URL_MAP",
+      "LEAN_SYSROOT", "LEAN_AR", "LEAN_PATH", "LEAN_SRC_PATH",
+      "ELAN_TOOLCHAIN", "DYLD_LIBRARY_PATH", "LD_LIBRARY_PATH"]
+
+
+  let cmd := "elan"
+  let args := #["run", "--install", toolchain, "lake", "exe", "subverso-extract-mod", mod]
+  let res ← IO.Process.output {
+    cmd, args, cwd := projectDir
+    -- Unset Lake's environment variables
+    env := lakeVars.map (·, none)
+  }
+  if res.exitCode != 0 then reportFail projectDir cmd args res
+  let output := res.stdout
+
+  let .ok (.arr json) := Lean.Json.parse output
+    | throw <| IO.userError s!"Expected JSON array"
+  match json.mapM fromJson? with
+  | .error err =>
+    throw <| IO.userError s!"Couldn't parse JSON from output file: {err}\nIn:\n{json}"
+  | .ok vals =>
+    pure vals
+
+
+where
+  decorateOut (name : String) (out : String) : String :=
+    if out.isEmpty then "" else s!"\n{name}:\n{out}\n"
+  reportFail {α} (projectDir : FilePath) (cmd : String) (args : Array String) (res : IO.Process.Output) : IO α := do
+    IO.eprintln <|
+      "Build process failed." ++
+      "\nCWD: " ++ projectDir.toString ++
+      "\nCommand: " ++ cmd ++
+      "\nArgs: " ++ repr args ++
+      "\nExit code: " ++ toString res.exitCode ++
+      "\nstdout: " ++ res.stdout ++
+      "\nstderr: " ++ res.stderr
+
+    throw <| .userError <|
+      "Build process failed." ++
+      decorateOut "stdout" res.stdout ++
+      decorateOut "stderr" res.stderr
+
+
+def desiredAnchors : List (String × String) := [
+  ("cons", "  | cons : Nat → NatList → NatList\n"),
+  ("NatList", "inductive NatList where\n  | nil\n  | cons : Nat → NatList → NatList\n")
+]
+def desiredProofs : List (String × String) := [
+  ("base", "case cons =>\n  ys: NatList\n  a✝¹: Nat\n  a✝: NatList\n  a_ih✝: ∀ (zs : NatList), a✝.append (ys.append zs) = (a✝.append ys).append zs\n⊢ ∀ (zs : NatList), (cons a✝¹ a✝).append (ys.append zs) = ((cons a✝¹ a✝).append ys).append zs"),
+  ("ind", "case nil =>\n  ys: NatList\n⊢ ∀ (zs : NatList), nil.append (ys.append zs) = (nil.append ys).append zs\n\ncase cons =>\n  ys: NatList\n  a✝¹: Nat\n  a✝: NatList\n  a_ih✝: ∀ (zs : NatList), a✝.append (ys.append zs) = (a✝.append ys).append zs\n⊢ ∀ (zs : NatList), (cons a✝¹ a✝).append (ys.append zs) = ((cons a✝¹ a✝).append ys).append zs"),
+  ("doubleIntro", "  xs: NatList\n  ys: NatList\n⊢ ∀ (zs : NatList), xs.append (ys.append zs) = (xs.append ys).append zs"),
+  ("step", "case cons =>\n  ys: NatList\n  a✝¹: Nat\n  a✝: NatList\n  a_ih✝: ∀ (zs : NatList), a✝.append (ys.append zs) = (a✝.append ys).append zs\n⊢ ∀ (zs : NatList), cons a✝¹ (a✝.append (ys.append zs)) = cons a✝¹ ((a✝.append ys).append zs)"),
+  ("ih", "case cons =>\n  ys: NatList\n  a✝¹: Nat\n  a✝: NatList\n  ih: ∀ (zs : NatList), a✝.append (ys.append zs) = (a✝.append ys).append zs\n⊢ ∀ (zs : NatList), cons a✝¹ (a✝.append (ys.append zs)) = cons a✝¹ ((a✝.append ys).append zs)"),
+  ("done", "")
+]
 
 def main : IO UInt32 := do
   IO.println "Checking the slice log"
@@ -181,6 +261,33 @@ def main : IO UInt32 := do
     IO.eprintln "No examples found"
     return 1
   else IO.println s!"Found {proofCount examplesToml} proofs"
+
+  IO.println "Checking anchor test file in TOML project"
+  cleanupDemo (demo := "demo-toml")
+  let anchorMod := (← loadModuleContent "demo-toml" "Anchors").map (·.code) |>.foldl (· ++ ·) (.empty)
+  match anchorMod.anchored with
+  | .error e => IO.eprintln e; return 1
+  | .ok {anchors, proofStates} =>
+    for k in desiredAnchors.map (·.1) do
+      unless anchors.contains k do IO.eprintln s!"Missing anchor '{k}'"; return 1
+    for k in desiredProofs.map (·.1) do
+      unless proofStates.contains k do IO.eprintln s!"Missing proofs state '{k}'"; return 1
+    for ⟨a, hl⟩ in anchors.toArray do
+      match desiredAnchors.lookup a with
+      | none => IO.eprintln s!"Unwanted anchor '{a}'"; return 1
+      | some s =>
+        if s ≠ hl.toString then
+          IO.eprintln s!"For anchor '{a}' expected\n{repr s}\nbut got\n{repr hl.toString}"; return 1
+    for ⟨p, y⟩ in proofStates.toArray do
+      if let .tactics info _s _e _ := y then
+        let g := info.map (·.toString) |>.toList |> String.intercalate "\n\n"
+        match desiredProofs.lookup p with
+        | none => IO.eprintln s!"Unwanted proof state '{p}'"; return 1
+        | some y' =>
+          if g ≠ y' then
+            IO.eprintln s!"For proof state '{p}' expected\n{repr y'}\nbut got\n{repr g}"; return 1
+      else
+        IO.eprintln "Got non-tactic {hl y}"; return 1
 
   IO.println "Checking that the test project generates at least some deserializable JSON with 4.3.0"
   cleanupDemo
