demo-toml/Anchors.lean
@@ -1,0 +1,31 @@
+/-
+Copyright (c) 2025 Lean FRO LLC. All rights reserved.
+Released under Apache 2.0 license as described in the file LICENSE.
+Author: David Thrane Christiansen
+-/
+
+-- ANCHOR: NatList
+inductive NatList where
+  | nil
+  --ANCHOR: cons
+  | cons : Nat → NatList → NatList
+  --ANCHOR_END: cons
+-- ANCHOR_END: NatList
+
+def NatList.append : NatList → NatList → NatList
+  | .nil, ys => ys
+  | .cons x xs, ys => .cons x (xs.append ys)
+
+theorem NatList.append_assoc : ∀ (xs ys zs : NatList), xs.append (ys.append zs) = (xs.append ys).append zs := by
+  intro xs ys
+  --^ PROOF_STATE: doubleIntro
+  induction xs
+  --^ PROOF_STATE: ind
+  simp [append]
+  --^ PROOF_STATE: base
+  simp only [append]
+  --^ PROOF_STATE: step
+  rename_i ih
+  --^ PROOF_STATE: ih
+  simp_all
+  --^ PROOF_STATE: done
