src/SubVerso/Highlighting.lean
@@ -5,3 +5,5 @@ Author: David Thrane Christiansen
 -/
 import SubVerso.Highlighting.Highlighted
 import SubVerso.Highlighting.Code
+import SubVerso.Highlighting.Anchors
+import SubVerso.Highlighting.String
