src/SubVerso/Highlighting/String.lean
@@ -1,0 +1,77 @@
+/-
+Copyright (c) 2025 Lean FRO LLC. All rights reserved.
+Released under Apache 2.0 license as described in the file LICENSE.
+Author: David Thrane Christiansen
+-/
+import SubVerso.Highlighting.Highlighted
+import SubVerso.Highlighting.Anchors
+import SubVerso.Compat
+
+namespace SubVerso.Highlighting.Highlighted
+
+/--
+Finds the first name `Token` whose string representation matches the given name exactly.
+
+Name tokens are those with kind `const` or `var`.
+-/
+partial def matchingName? (hl : Highlighted) (name : String) : Option Token := do
+  match hl with
+  | .seq xs => xs.findSome? (matchingName? · name)
+  | .point .. | .text .. => none
+  | .tactics _ _ _ x | .span _ x => matchingName? x name
+  | .token t@⟨k, s⟩ =>
+    match k with
+    | .const .. | .var .. => if s == name then return t else none
+    | _ => none
+
+/--
+Splits highlighted code into its first token followed by the rest of the code. If the code doesn't
+begin with a `.token`, `none` is returned.
+-/
+partial def firstToken (hl : Highlighted) : Option (Highlighted × Highlighted) :=
+  match hl with
+  | .seq xs => do
+    let mut xs := xs
+    repeat
+      if let some x := xs[0]? then
+        xs := xs.extract 1 xs.size
+        if let some (t, xs') := firstToken x then
+          return (t, xs' ++ .seq xs)
+        else continue
+      else failure
+    failure
+  | .point .. | .text .. => none
+  | .tactics _ _ _ x | .span _ x => firstToken x
+  | .token .. => pure (hl, .empty)
+
+/--
+Returns the prefix of `hl` that matches the string `term`. The returned code has whitespace from
+`term`.
+-/
+def matchingExprPrefix? (hl : Highlighted) (term : String) : Option Highlighted := do
+  let mut out : Highlighted := .empty
+  let mut term := term
+  let mut hl := hl
+  while !term.isEmpty do
+    let ws := term.takeWhile (·.isWhitespace)
+    out := out ++ .text ws
+    term := term.trimLeft
+    let (first, rest) ← firstToken hl
+    hl := rest
+    let firstStr := first.toString
+    let term' ← term.dropPrefix? firstStr
+    term := term'.toString
+    out := out ++ first
+  return out
+
+/--
+Returns the first subsequence of `hl` that matches the string `term`. The returned code has
+whitespace from `term`.
+-/
+def matchingExpr? (hl : Highlighted) (term : String) : Option Highlighted := do
+  let mut hl := hl
+  repeat
+    let (first, rest) ← firstToken hl
+    if let some out := matchingExprPrefix? (first ++ rest) term then return out
+    else hl := rest
+  failure
